renamings, prep for lift

examples/dm4free/intST.fst
@@ -1,104 +1,104 @@
 module IntST
 
-let st_pre = int -> Type0
-let st_post (a:Type) = (a * int) -> Type0
-let st_wp (a:Type) = int -> st_post a -> Type0
+let pre = int -> Type0
+let post (a:Type) = (a * int) -> Type0
+let wp (a:Type) = int -> post a -> Type0
 assume val r0: range
-inline let st_return_wp (a:Type) (x:a) (n0:int) (post:st_post a) = 
+inline let return_wp (a:Type) (x:a) (n0:int) (post:post a) = 
   forall y. y=(x, n0) ==> post y
 
 //working around #517 by adding an explicit 'val'
-inline val st_bind_wp : r:range -> (a:Type) -> (b:Type) -> (f:st_wp a) -> (g:(a -> Tot (st_wp b))) -> Tot (st_wp b)
-let st_bind_wp r a b f g =
+inline val bind_wp : r:range -> (a:Type) -> (b:Type) -> (f:wp a) -> (g:(a -> Tot (wp b))) -> Tot (wp b)
+let bind_wp r a b f g =
     fun n0 post -> f n0 (fun x_n1 -> g (fst x_n1) (snd x_n1) post)
 
-inline let st_if_then_else  (a:Type) (p:Type)
-                            (wp_then:st_wp a) (wp_else:st_wp a)
-                            (h0:int) (post:st_post a) =
+inline let if_then_else  (a:Type) (p:Type)
+                            (wp_then:wp a) (wp_else:wp a)
+                            (h0:int) (post:post a) =
      l_ITE p
         (wp_then h0 post)
 	(wp_else h0 post)
-inline let st_ite_wp        (a:Type)
-                            (wp:st_wp a)
-                            (h0:int) (post:st_post a) =
-     forall (k:st_post a).
-	 (forall (x:a) (h:int).{:pattern (guard_free (k (x, h)))} k (x, h) <==> post (x, h))
+inline let ite_wp        (a:Type)
+                            (wp:wp a)
+                            (h0:int) (q:post a) =
+     forall (k:post a).
+	 (forall (x:a) (h:int).{:pattern (guard_free (k (x, h)))} k (x, h) <==> q (x, h))
 	 ==> wp h0 k
-inline let st_stronger  (a:Type) (wp1:st_wp a) (wp2:st_wp a) =
-     (forall (p:st_post a) (h:int). wp1 h p ==> wp2 h p)
+inline let stronger  (a:Type) (wp1:wp a) (wp2:wp a) =
+     (forall (p:post a) (h:int). wp1 h p ==> wp2 h p)
 
-inline let st_close_wp      (a:Type) (b:Type)
-                            (wp:(b -> GTot (st_wp a)))
-                            (h:int) (p:st_post a) =
+inline let close_wp      (a:Type) (b:Type)
+                            (wp:(b -> GTot (wp a)))
+                            (h:int) (p:post a) =
      (forall (b:b). wp b h p)
-inline let st_assert_p      (a:Type) (p:Type)
-                            (wp:st_wp a)
-                            (h:int) (q:st_post a) =
+inline let assert_p      (a:Type) (p:Type)
+                            (wp:wp a)
+                            (h:int) (q:post a) =
      p /\ wp h q
-inline let st_assume_p      (a:Type) (p:Type)
-                            (wp:st_wp a)
-                            (h:int) (q:st_post a) =
+inline let assume_p      (a:Type) (p:Type)
+                            (wp:wp a)
+                            (h:int) (q:post a) =
      p ==> wp h q
-inline let st_null_wp       (a:Type)
-                            (h:int) (p:st_post a) =
+inline let null_wp       (a:Type)
+                            (h:int) (p:post a) =
      (forall (x:a) (h:int). p (x,h))
-inline let st_trivial       (a:Type)
-                            (wp:st_wp a) =
+inline let trivial       (a:Type)
+                            (wp:wp a) =
      (forall h0. wp h0 (fun r -> True))
 
 //new
-let st_repr (a:Type) (wp:st_wp a) =
+let repr (a:Type) (wp:wp a) =
     n0:int -> PURE (a * int) (wp n0)
 
-inline val st_bind: (a:Type) -> (b:Type) -> (wp0:st_wp a) -> (wp1:(a -> Tot (st_wp b))) 
-		 -> (f:st_repr a wp0)
-		 -> (g:(x:a -> Tot (st_repr b (wp1 x)))) 
-		 -> Tot (st_repr b (st_bind_wp r0 a b wp0 wp1))
-let st_bind a b wp0 wp1 f g  
+inline val bind: (a:Type) -> (b:Type) -> (wp0:wp a) -> (wp1:(a -> Tot (wp b))) 
+		 -> (f:repr a wp0)
+		 -> (g:(x:a -> Tot (repr b (wp1 x)))) 
+		 -> Tot (repr b (bind_wp r0 a b wp0 wp1))
+let bind a b wp0 wp1 f g  
   = fun n0 -> admit(); let (x,n1) = f n0 in g x n1
-let st_return (a:Type) (x:a)
-  : st_repr a (st_return_wp a x)
+let return (a:Type) (x:a)
+  : repr a (return_wp a x)
   = fun n0 -> (x, n0)
 
-let st_get (u:unit) : st_repr int (fun n0 post -> post (n0, n0))
+let get (u:unit) : repr int (fun n0 post -> post (n0, n0))
   = fun n0 -> n0, n0
 
-let st_put (n:int) : st_repr unit (fun n0 post -> post ((), n))
+let put (n:int) : repr unit (fun n0 post -> post ((), n))
   = fun x -> (), n
 
 (* //#reset-options "--debug NatST --debug_level SMTEncoding" *)
 
 reifiable reflectable new_effect {
-  STATE : a:Type -> wp:st_wp a -> Effect
+  STATE : a:Type -> wp:wp a -> Effect
   with //repr is new; it's the reprentation of ST as a value type
-       repr         = st_repr
+       repr         = repr
        //bind_wp is exactly as it is currently
        //produced by the *-translation of bind above
-     ; bind_wp      = st_bind_wp
+     ; bind_wp      = bind_wp
        //bind is new, it is the elaboration of the bind above
-     ; bind         = st_bind
+     ; bind         = bind
       //return_wp is a renaming of the current return, it is the *-translation of the return above
-     ; return_wp    = st_return_wp
+     ; return_wp    = return_wp
       //return is new; it is the elaboration of the return above
-     ; return       = st_return
+     ; return       = return
      //the remaining are just as what we have now
-     ; if_then_else = st_if_then_else
-     ; ite_wp       = st_ite_wp
-     ; stronger     = st_stronger
-     ; close_wp     = st_close_wp
-     ; assert_p     = st_assert_p
-     ; assume_p     = st_assume_p
-     ; null_wp      = st_null_wp
-     ; trivial      = st_trivial
+     ; if_then_else = if_then_else
+     ; ite_wp       = ite_wp
+     ; stronger     = stronger
+     ; close_wp     = close_wp
+     ; assert_p     = assert_p
+     ; assume_p     = assume_p
+     ; null_wp      = null_wp
+     ; trivial      = trivial
   and effect_actions
     //these are new
-      get  = st_get
-    ; put  = st_put
+      get  = get
+    ; put  = put
 }
-inline let lift_pure_state (a:Type) (wp:pure_wp a) (n:int) (p:st_post a) = wp (fun a -> p (a, n))
+inline let lift_pure_state (a:Type) (wp:pure_wp a) (n:int) (p:post a) = wp (fun a -> p (a, n))
 sub_effect PURE ~> STATE = lift_pure_state
 
-effect ST (a:Type) (pre:st_pre) (post: (int -> a -> int -> GTot Type0)) =
+effect ST (a:Type) (pre:pre) (post: (int -> a -> int -> GTot Type0)) =
        STATE a
              (fun n0 p -> pre n0 /\ (forall a n1. pre n0 /\ post n0 a n1 ==> p (a, n1)))
 
@@ -128,7 +128,7 @@ let f (_:unit) : St unit =
 val g : unit -> St int
 let g u =
     let n0 = STATE.get () in
-    let f : st_repr unit (fun n0 post -> forall x. snd x=n0+2 ==> post x) =
+    let f : repr unit (fun n0 post -> forall x. snd x=n0+2 ==> post x) =
       fun n0 -> (), n0+2 in
     STATE.reflect f;
     let n1 = STATE.get () in
@@ -140,21 +140,21 @@ let top =
   FStar.IO.print_string ("incr2 returned: " ^ string_of_int one)
 
 (* (\* sub_effect PURE ~> STATE { *\) *)
-(* (\*   lift_wp: #a:Type -> #wp:pure_wp a -> st_wp a = ... *\) *)
+(* (\*   lift_wp: #a:Type -> #wp:pure_wp a -> wp a = ... *\) *)
 (* (\*   lift   : #a:Type -> #wp:pure_wp a -> f:PURE.repr a wp -> STATE.repr a (lift_star wp) = ... *\) *)
 (* (\* }   *\) *)
 
 (* (\* //////////////////////////////////////////////////////////////////////////////// *\) *)
-(* (\* (\\* let repr_STATE (a:Type) (wp:st_wp a) =  *\\) *\) *)
+(* (\* (\\* let repr_STATE (a:Type) (wp:wp a) =  *\\) *\) *)
 (* (\* (\\*   n0:nat -> PURE (a * nat) (fun post -> wp (fun a n -> post (a, n)) n0) *\\) *\) *)
 
 
 
 (* (\* new_effect STATE = STATE_h nat *\) *)
-(* (\* let st_pre = st_pre_h nat *\) *)
-(* (\* let st_post a = st_post_h nat a *\) *)
-(* (\* let st_wp a = st_wp_h nat a *\) *)
-(* (\* inline let lift_pure_state (a:Type) (wp:pure_wp a) (p:st_post a) (n:nat) = wp (fun a -> p a n) *\) *)
+(* (\* let pre = pre_h nat *\) *)
+(* (\* let post a = poh nat a *\) *)
+(* (\* let wp a = wp_h nat a *\) *)
+(* (\* inline let lift_pure_state (a:Type) (wp:pure_wp a) (p:post a) (n:nat) = wp (fun a -> p a n) *\) *)
 (* (\* sub_effect PURE ~> STATE = lift_pure_state *\) *)
 
 (* (\* let reify_STATE (a:Type) = nat -> Tot (a * nat) *\) *)
@@ -185,17 +185,17 @@ let top =
 
 
 
-(* (\* (\\* let repr_STATE (a:Type) (wp:st_wp a) =  *\\) *\) *)
+(* (\* (\\* let repr_STATE (a:Type) (wp:wp a) =  *\\) *\) *)
 (* (\* (\\*   n0:nat -> PURE (a * nat) (fun post -> wp (fun a n -> post (a, n)) n0) *\\) *\) *)
 
-(* (\* (\\* inline let lift_pure_state (a:Type) (wp:pure_wp a) (p:st_post a) (n:nat) = wp (fun a -> p a n) *\\) *\) *)
+(* (\* (\\* inline let lift_pure_state (a:Type) (wp:pure_wp a) (p:post a) (n:nat) = wp (fun a -> p a n) *\\) *\) *)
 (* (\* (\\* sub_effect PURE ~> STATE = lift_pure_state *\\) *\) *)
 (* (\* (\\* assume val r : range *\\) *\) *)
 
-(* (\* (\\* val repr_bind: #a:Type -> #b:Type -> #wp1:st_wp a -> #wp2:(a -> GTot (st_wp b)) *\\) *\) *)
+(* (\* (\\* val repr_bind: #a:Type -> #b:Type -> #wp1:wp a -> #wp2:(a -> GTot (wp b)) *\\) *\) *)
 (* (\* (\\* 	     -> repr_STATE a wp1 *\\) *\) *)
 (* (\* (\\* 	     -> (x:a -> Tot (repr_STATE b (wp2 x))) *\\) *\) *)
-(* (\* (\\* 	     -> Tot (repr_STATE b (st_bind_wp nat r a b wp1 wp2)) *\\) *\) *)
+(* (\* (\\* 	     -> Tot (repr_STATE b (bind_wp nat r a b wp1 wp2)) *\\) *\) *)
 (* (\* (\\* #reset-options "--log_queries"	      *\\) *\) *)
 (* (\* (\\* let repr_bind #a #b #wp1 #wp2 f g =  *\\) *\) *)
 (* (\* (\\*   fun n0 -> admit(); //the encoding to SMT isn't sufficiently smart to capture monotonicity *\\) *\) *)
